\documentclass[a4paper]{article}
\usepackage{amsmath}
\begin{document}
 \(\int_{0}^{1} c(x+a) \,dx\) = 1
 

  \(c\int_{0}^{1} (x+a) \,dx\ = c(\int_{0}^{1} x \,dx\ + 
  c\int_{0}^{1} a \,dx)\)
  
  
  \(\int x \, dx = \frac{x^2}{2}\)
  \(\int a \, dx = ax\)
  
	\( \)
	
	
  \(\left. c(\frac{x^2}{2} + ax)\right\vert_{0}^{1} = 
  c((\frac{1}{2} + a) - (\frac{0}{2} + 0)) = c(\frac{1}{2} + a)\)
  
  \(c(\frac{1}{2} + a) = 1\)
  
  \( c = \frac{1}{\frac{1}{2} + a} \)
  
  \( a = 1.1; c = \frac{1}{\frac{1}{2} + 1.1} = 0.625 \)
    
  \[ f(x) = \begin{cases} 
      0 & x < 0 \\
      0.625 x + 0.6875 & 0\leq x\leq 1 \\
      0 & 1 < x 
   \end{cases}
\]


\end{document}
